proofs.v
@@ -1,0 +1,40 @@
+Require Export init.
+Require Import univ examples.
+
+(* simple proofs about self-defined generic types *)
+
+Theorem sum_eq_teither (A B : Type)
+  : sum A B = decodeClosed teither A B.
+Proof.
+  unfold decodeClosed; unfold decodeType; simpl.
+  reflexivity.
+Qed.
+
+Definition optMaybe (A : Type) (o : option A) : decodeClosed tmaybe A :=
+  match o with
+  | Some x => inr x
+  | None => inl tt
+  end.
+
+Definition maybeOpt (A : Type) (t : decodeClosed tmaybe A) : option A :=
+  match t with
+  | inl tt => None
+  | inr x => Some x
+  end.
+
+Theorem opt_eq_tmaybe (A : Type) (o : option A)
+  : maybeOpt (optMaybe o) = o.
+Proof.
+  destruct o as [sa |].
+  - reflexivity.
+  - reflexivity.
+Qed.
+
+Theorem tmaybe_eq_opt (A : Type) (m : decodeClosed tmaybe A)
+  : optMaybe (maybeOpt m) = m.
+Proof.
+  destruct m as [sm |].
+  - destruct sm; reflexivity.
+  - reflexivity.
+Qed.
+
